Big cleanup: merge redux and non-redux
- Still a bunch of TODO's (verification broken in TLSConstants.fst)
- A weird extraction error in MAC_SHA1.fst (see comment)
- Cleanup up the Makefile, changed targets and shared variables between
  verification, testing and extraction.

src/tls/TLSConstants.fst
@@ -83,6 +83,7 @@ type sigAlg = CoreCrypto.sig_alg
 
 type sigHashAlg = sigAlg * hashAlg
 
+
 (* Serializing function for signature algorithms *)
 val sigAlgBytes: sigAlg -> Tot (lbytes 1)
 let sigAlgBytes sa =
@@ -92,9 +93,16 @@ let sigAlgBytes sa =
     | CoreCrypto.ECDSA  -> abyte 3uy
     | CoreCrypto.RSAPSS -> abyte 4uy
 
-type pinverse_t (#a:Type) (#b:Type) (=f:(a -> Tot b)) = 
+(* This is the old version of the inverse predicate. According to CF,
+   verification was harder with this style, so we moved to the new style with
+   pinverse_t + lemmas. The type abbrevations lemma_inverse_* minimize the
+   syntactic overhead. *)
+(* logic type pinverse (#a:Type) (#b:Type) (r:(b -> b -> Type)) (=f:(a -> Tot b)) =
+    (y:b -> Tot (xopt:Result a{(forall (x:a). r (f x) y <==> (xopt = Correct x))})) *)
+
+type pinverse_t (#a:Type) (#b:Type) (=f:(a -> Tot b)) =
     (y:b -> Tot (Result a))
- 
+
 (* Parsing function associated to sigAlgBytes *)
 val parseSigAlg: pinverse_t sigAlgBytes
 let parseSigAlg b =
@@ -110,7 +118,7 @@ type lemma_inverse_g_f (#a:Type) (#b:Type) (=f:(a -> Tot b)) (=g:(b -> Tot (Resu
 
 type lemma_pinverse_f_g (#a:Type) (#b:Type) (r:b -> b -> Type) (=f:(a -> Tot b)) (=g:(b -> Tot (Result a))) (y:b) =
   is_Correct (g y) ==> r (f (Correct._0 (g y))) y
- 
+
 val inverse_sigAlg: x:_ -> Lemma
   (requires (True)) 
   (ensures lemma_inverse_g_f sigAlgBytes parseSigAlg x)
@@ -123,8 +131,8 @@ val pinverse_sigAlg: x:_ -> Lemma
   [SMTPat (sigAlgBytes (Correct._0 (parseSigAlg x)))]
 let pinverse_sigAlg x = ()
 
-type hashAlg' = h:hashAlg{h <> NULL /\ h <> MD5SHA1 } 
- 
+type hashAlg' = h:hashAlg{h <> NULL /\ h <> MD5SHA1 }
+
 val hashAlgBytes : hashAlg' -> Tot (lbytes 1)
 let hashAlgBytes ha =
     match ha with
@@ -138,12 +146,12 @@ let hashAlgBytes ha =
 val parseHashAlg: pinverse_t hashAlgBytes
 let parseHashAlg b =
     match cbyte b with
-    | (1uy) -> Correct (Hash MD5)
-    | (2uy) -> Correct (Hash SHA1)
-    | (3uy) -> Correct (Hash SHA224)
-    | (4uy) -> Correct (Hash SHA256)
-    | (5uy) -> Correct (Hash SHA384)
-    | (6uy) -> Correct (Hash SHA512)
+    | 1uy -> Correct (Hash MD5)
+    | 2uy -> Correct (Hash SHA1)
+    | 3uy -> Correct (Hash SHA224)
+    | 4uy -> Correct (Hash SHA256)
+    | 5uy -> Correct (Hash SHA384)
+    | 6uy -> Correct (Hash SHA512)
     | _ -> Error (AD_decode_error, perror __SOURCE_FILE__ __LINE__ "")
 
 val inverse_hashAlg: x:_ -> Lemma
@@ -256,7 +264,7 @@ let parseVersion v =
     | ( 3uy, 2uy ) -> Correct(TLS_1p1)
     | ( 3uy, 3uy ) -> Correct(TLS_1p2)
     | ( 3uy, 4uy ) -> Correct(TLS_1p3)
-    | _ -> Error(AD_decode_error, perror __SOURCE_FILE__ __LINE__ "")
+    | _ -> Error(AD_decode_error, perror __SOURCE_FILE__ __LINE__ "Parsed an unknown version")
 
 val inverse_version: x:_ -> Lemma
   (requires (True)) 
@@ -457,7 +465,7 @@ let parseCipherSuiteAux b =
 
     | ( 0x00uy, 0xFFuy ) -> Correct(SCSV (TLS_EMPTY_RENEGOTIATION_INFO_SCSV))
 
-    | _ -> Error(AD_decode_error, perror __SOURCE_FILE__ __LINE__ "")
+    | _ -> Error(AD_decode_error, perror __SOURCE_FILE__ __LINE__ "Parsed unknown cipher")
 
 val parseCipherSuite : pinverse_t cipherSuiteBytes
 let parseCipherSuite b =
@@ -500,7 +508,7 @@ let rec parseCipherSuites b : Result known_cipher_suites =
              | Correct(cs) -> Correct(cs::css))
          | Error(z) -> Error(z)
      else if length b = 0 then Correct []
-     else Error(AD_decode_error, perror __SOURCE_FILE__ __LINE__ "")
+     else Error(AD_decode_error, perror __SOURCE_FILE__ __LINE__ "Odd cs bytes number")
 
 val cipherSuitesBytes: css:known_cipher_suites -> Tot (lbytes (2 * List.length css))
 let rec cipherSuitesBytes css =
@@ -973,3 +981,348 @@ let contains_TLS_EMPTY_RENEGOTIATION_INFO_SCSV (css: list cipherSuite) =
     List.mem (SCSV (TLS_EMPTY_RENEGOTIATION_INFO_SCSV)) css
 
 // let test_me () = assert False
+(* TODO: move all the definitions below to a separate file / figure out whether
+ they belong here? *)
+(* TODO: all occurrences of [pinverse] from there on have been replaced by calls
+ to [pinverse_t]; we should write corresponding inversion lemmas. *)
+
+type ffdhe =
+  | FFDHE2048
+  | FFDHE3072
+  | FFDHE4096
+  | FFDHE6144
+  | FFDHE8192
+
+(* TLS 1.3 constants *)
+type namedGroup =
+  | SEC of CoreCrypto.ec_curve
+  | EC_UNSUPPORTED of byte
+  | FFDHE of ffdhe
+  | FFDHE_PRIVATE_USE of byte // fist byte is fixed 
+  | ECDHE_PRIVATE_USE of byte // fist byte is fixed
+
+val namedGroupBytes: namedGroup -> Tot (lbytes 2)
+let namedGroupBytes ng =
+  match ng with
+  | SEC(ec) ->
+    (match ec with
+    | ECC_P256                      -> abyte2 (0x00uy, 0x17uy)
+    | ECC_P384                      -> abyte2 (0x00uy, 0x18uy)
+    | ECC_P521                      -> abyte2 (0x00uy, 0x19uy))
+  | EC_UNSUPPORTED(b)               -> abyte2 (0x00uy, b)
+  | FFDHE(dhe) ->
+    (match dhe with
+    | FFDHE2048                     -> abyte2 (0x01uy, 0x00uy)
+    | FFDHE3072                     -> abyte2 (0x01uy, 0x01uy)
+    | FFDHE4096                     -> abyte2 (0x01uy, 0x02uy))
+  | FFDHE_PRIVATE_USE(b)            -> abyte2 (0x01uy, b) 
+  | ECDHE_PRIVATE_USE(b)            -> abyte2 (0xFEuy, b)
+
+val parseNamedGroup: pinverse_t namedGroupBytes
+let parseNamedGroup b =
+  match cbyte2 b with
+  | (0x00uy, 0x17uy) -> Correct (SEC(ECC_P256))
+  | (0x00uy, 0x18uy) -> Correct (SEC(ECC_P384))
+  | (0x00uy, 0x19uy) -> Correct (SEC(ECC_P521))
+  | (0x00uy, x) -> let v = int_of_bytes (abyte x) in
+		   (*if v > 0 && v < 17 then *) Correct(EC_UNSUPPORTED (x))
+//		   else Error (AD_decode_error, perror __SOURCE_FILE__ __LINE__ "Wrong ec named group")
+  | (0x01uy, 0x00uy) -> Correct (FFDHE(FFDHE2048))
+  | (0x01uy, 0x01uy) -> Correct (FFDHE(FFDHE3072))
+  | (0x01uy, 0x02uy) -> Correct (FFDHE(FFDHE4096))
+  | (0x01uy, 0x03uy) -> Correct (FFDHE(FFDHE6144))
+  | (0x01uy, 0x04uy) -> Correct (FFDHE(FFDHE8192))
+  | (0x01uy, v)      -> if v = 0xFCuy || v = 0xFDuy || v = 0xFEuy || v = 0xFFuy 
+			then Correct (FFDHE_PRIVATE_USE v)
+			else Error (AD_decode_error, perror __SOURCE_FILE__ __LINE__ "Wrong ffdhe private use group")
+  | (0xFEuy, v)      -> Correct (ECDHE_PRIVATE_USE v)
+  | _ -> Error (AD_decode_error, perror __SOURCE_FILE__ __LINE__ "Wrong named group")
+
+val namedGroupsBytes: list namedGroup -> Tot bytes
+let namedGroupsBytes groups =
+  vlbytes 2 (List.Tot.fold_left (fun l s -> namedGroupBytes s @| l) empty_bytes groups)
+
+val parseNamedGroups: pinverse_t namedGroupsBytes
+let parseNamedGroups b =
+  let rec (aux:bytes -> list namedGroup -> Tot (Result (list namedGroup))) = fun b groups ->
+    if length b > 0 then
+      if length b >= 2 then
+	let (ng, bytes) = split b 2 in
+	match parseNamedGroup ng with
+	| Correct(ng) -> aux bytes (ng::groups)
+	| Error(z) -> Error(z)
+      else Error (AD_decode_error, perror __SOURCE_FILE__ __LINE__ "")
+    else Correct(groups) in      
+  match vlparse 2 b with
+  | Correct(b) -> aux b []
+  | Error(z) -> Error(AD_decode_error, perror __SOURCE_FILE__ __LINE__ "Failed to parse named groups")
+
+(* TODO : precise configurationId type *)
+type configurationId = b:bytes{not (equalBytes b empty_bytes) /\ length b < 65536}
+
+val configurationIdBytes: configurationId -> Tot bytes
+let configurationIdBytes cid = vlbytes 2 cid
+
+val parseConfigurationId: pinverse_t configurationIdBytes
+let parseConfigurationId b = vlparse 2 b
+
+type uint32 = b:lbytes 4
+
+val uint32Bytes: uint32 -> Tot (lbytes 4)
+let uint32Bytes u = u
+
+val parseUint32: pinverse_t uint32Bytes
+let parseUint32 b =
+  if length b = 4 then Correct(b)
+  else Error (AD_decode_error, perror __SOURCE_FILE__ __LINE__ "")
+
+type earlyDataType =
+  | ClientAuthentication
+  | EarlyData
+  | ClientAuthenticationAndData
+
+val earlyDataTypeBytes : earlyDataType -> Tot (lbytes 1)
+let earlyDataTypeBytes edt =
+  match edt with
+  | ClientAuthentication          -> abyte 1uy
+  | EarlyData                     -> abyte 2uy
+  | ClientAuthenticationAndData   -> abyte 3uy
+
+val parseEarlyDataType: pinverse_t earlyDataTypeBytes
+let parseEarlyDataType b =
+    match cbyte b with
+    | (1uy) -> Correct (ClientAuthentication)
+    | (2uy) -> Correct (EarlyData)
+    | (3uy) -> Correct (ClientAuthenticationAndData)
+    | _ -> Error (AD_decode_error, perror __SOURCE_FILE__ __LINE__ "Failed to parse early data type")
+
+// TODO : replace with more precise types when available
+type configurationExtension =
+  | UnknownConfigurationExtension of lbytes 2 * bytes
+
+val configurationExtensionBytes: configurationExtension -> Tot bytes
+let configurationExtensionBytes ce = 
+  match ce with 
+  | UnknownConfigurationExtension(typ, payload) -> typ @| vlbytes 2 payload
+
+val parseConfigurationExtension: pinverse_t configurationExtensionBytes
+let parseConfigurationExtension b = 
+  if length b >= 2 then
+    let (typ, payload) = split b 2 in
+    match vlparse 2 payload with
+    | Correct (payload) -> Correct (UnknownConfigurationExtension(typ, payload))
+    | Error(z) -> Error(z)
+  else Error (AD_decode_error, perror __SOURCE_FILE__ __LINE__ "Too few bytes to parse a configuration extension")
+
+val configurationExtensionsBytes: list configurationExtension -> Tot bytes
+let configurationExtensionsBytes ce = 
+  vlbytes 2 (List.Tot.fold_left (fun bytes x -> bytes @| configurationExtensionBytes x) empty_bytes ce)
+
+val parseConfigurationExtensions: pinverse_t configurationExtensionsBytes
+let parseConfigurationExtensions b = 
+  let rec (aux:bytes -> list configurationExtension -> Tot (Result (list configurationExtension))) =
+    fun b exts ->
+    if length b > 0 then
+      if length b >= 4 then
+	let typ, len, data = split2 b 2 2 in
+	let len = int_of_bytes len in
+	if length b >= 4 + len then
+	  let ext, bytes = split b len in
+	  match parseConfigurationExtension ext with
+	  | Correct(ext') -> aux bytes (ext'::exts)
+	  | Error(z) -> Error(z)
+	else Error(AD_decode_error, perror __SOURCE_FILE__ __LINE__ "Failed to parse configuration extension length")
+      else Error(AD_decode_error, perror __SOURCE_FILE__ __LINE__ "Configuration extension length should be at least 4")
+    else Correct(exts) in
+  match vlparse 2 b with
+  | Correct (b) ->  aux b []
+  | Error(z) -> Error(AD_decode_error, perror __SOURCE_FILE__ __LINE__ "Failed to parse configuration extension")
+
+val sigHashAlgBytes: sigHashAlg -> Tot (lbytes 2)
+let sigHashAlgBytes sha =
+  let sign = sigAlgBytes (fst sha) in
+  let hash = hashAlgBytes (snd sha) in
+  hash @| sign
+
+val parseSigHashAlg: pinverse_t sigHashAlgBytes
+let parseSigHashAlg b =
+  if length b = 2 then
+    let (hash, sign) = split b 1 in
+    match parseSigAlg sign with
+    | Correct(sign) -> 
+	(match parseHashAlg hash with
+	| Correct(hash) -> Correct(sign, hash)
+	| Error(z) -> Error(z))
+    | Error(z) -> Error(z)
+  else Error (AD_decode_error, perror __SOURCE_FILE__ __LINE__ "Remaining unparsed bytes after signature hash algorithm")
+
+val sigHashAlgsBytes: list sigHashAlg -> Tot bytes
+let sigHashAlgsBytes algs = 
+  vlbytes 2 (List.Tot.fold_left (fun l x -> sigHashAlgBytes x @| l) empty_bytes algs)
+
+val parseSigHashAlgs: pinverse_t sigHashAlgsBytes
+let parseSigHashAlgs b =
+  let rec (aux:bytes -> list sigHashAlg -> Tot (Result (list sigHashAlg))) = fun b algs ->
+    if length b > 0 then
+      if length b >= 2 then
+      let (alg, bytes) = split b 2 in
+      match parseSigHashAlg alg with
+      | Correct(sha) -> aux bytes (sha::algs)
+      | Error(z) -> Error(z)
+      else Error (AD_decode_error, perror __SOURCE_FILE__ __LINE__ "Too few bytes to parse sig hash algs")
+    else Correct(algs) in
+  match vlparse 2 b with
+  | Correct (b) -> aux b []
+  | Error(z) -> Error(AD_decode_error, perror __SOURCE_FILE__ __LINE__ "Failed to parse sig hash algs")
+
+// TODO : replace "bytes" by either DH or ECDH parameters
+type keyShareEntry = namedGroup * bytes
+
+val keyShareEntryBytes: keyShareEntry -> Tot bytes
+let keyShareEntryBytes kse =
+  let (ng, bytes) = kse in
+  let ng_bytes = namedGroupBytes ng in
+  ng_bytes @| vlbytes 2 bytes
+
+val parseKeyShareEntry: pinverse_t keyShareEntryBytes
+let parseKeyShareEntry b =
+  if length b >= 2 then
+    let ng, key_exchange = split b 2 in
+    match parseNamedGroup ng with
+    | Correct(ng) -> 
+	(match vlparse 2 key_exchange with
+	| Correct(ke) -> Correct (ng, ke)
+	| Error(z) -> Error(AD_decode_error, perror __SOURCE_FILE__ __LINE__ "Failed to parse key share entry"))
+    | Error(z) -> Error(z)
+  else Error (AD_decode_error, perror __SOURCE_FILE__ __LINE__ "Too few bytes to parse key share entry")
+
+val keyShareEntriesBytes: list keyShareEntry -> Tot bytes
+let keyShareEntriesBytes kses =
+  vlbytes 2 (List.Tot.fold_left (fun l s -> l @| keyShareEntryBytes s) empty_bytes kses)
+
+val parseKeyShareEntries: pinverse_t keyShareEntriesBytes
+let parseKeyShareEntries b =
+  let rec (aux:bytes -> list keyShareEntry -> Tot (Result (list keyShareEntry))) = fun b entries ->
+    if length b > 0 then
+      if length b >= 2 then
+	let (ng, data) = split b 2 in
+	match vlsplit 2 data with
+	| Correct(kex, bytes) -> 
+	    (match parseKeyShareEntry (ng @| vlbytes 2 kex) with
+	    | Correct(entry) -> aux bytes (entry::entries)
+	    | Error(z) -> Error(z))
+	| Error(z) -> Error(AD_decode_error, perror __SOURCE_FILE__ __LINE__ "Failed to parse key share entry")
+      else Error (AD_decode_error, perror __SOURCE_FILE__ __LINE__ "Too few bytes to parse key share entries")
+    else Correct(entries) in
+  match vlparse 2 b with
+  | Correct (b) ->  aux b []
+  | Error(z) -> Error(AD_decode_error, perror __SOURCE_FILE__ __LINE__ "Failed to parse key share entries")
+  
+type clientKeyShare = l:list keyShareEntry{List.length l >= 4 /\ List.length l < 65536}
+type serverKeyShare = keyShareEntry
+
+type keyShare = 
+  | ClientKeyShare of clientKeyShare
+  | ServerKeyShare of serverKeyShare
+
+val clientKeyShareBytes: clientKeyShare -> Tot bytes
+let clientKeyShareBytes cks = 
+  keyShareEntriesBytes cks
+
+val parseClientKeyShare: pinverse_t clientKeyShareBytes
+let parseClientKeyShare b = parseKeyShareEntries b
+
+val serverKeyShareBytes: serverKeyShare -> Tot bytes
+let serverKeyShareBytes sks =
+  keyShareEntryBytes sks
+
+val parseServerKeyShare: pinverse_t serverKeyShareBytes
+let parseServerKeyShare b = parseKeyShareEntry b
+
+val keyShareBytes: keyShare -> Tot bytes
+let keyShareBytes ks = 
+  match ks with
+  | ClientKeyShare cks -> clientKeyShareBytes cks
+  | ServerKeyShare sks -> serverKeyShareBytes sks
+
+(* TODO: FIXME *)
+val parseKeyShare: pinverse_t keyShareBytes
+let parseKeyShare b =
+  match parseKeyShareEntries b with
+  | Correct(kse) -> 
+      (match kse with
+      | e::[] -> Correct(ServerKeyShare e)
+      | _ -> if List.length kse >= 2 && List.length kse < 65536 then Correct(ClientKeyShare (kse))
+	     else Error (AD_decode_error, perror __SOURCE_FILE__ __LINE__ "Wrong key share length") )
+  | Error(z) -> Error(z)
+
+// TODO : give more precise type
+type pskIdentity = b:bytes{length b < 65536}
+
+val pskIdentityBytes: pskIdentity -> Tot bytes
+let pskIdentityBytes pski = vlbytes 2 (pski)
+
+val parsePskIdentity: pinverse_t pskIdentityBytes
+let parsePskIdentity b = vlparse 2 b
+
+val pskIdentitiesBytes: list pskIdentity -> Tot bytes
+let pskIdentitiesBytes l =
+  vlbytes 2 (List.Tot.fold_left (fun l s -> l @| pskIdentityBytes s) empty_bytes l)
+
+val parsePskIdentities: pinverse_t pskIdentitiesBytes
+let parsePskIdentities b =
+  let rec (aux: bytes -> list pskIdentity -> Tot (Result (list pskIdentity))) = fun b ids ->
+    if length b > 0 then
+      if length b >= 2 then
+	let len, data = split b 2 in
+	let len = int_of_bytes len in
+	if length b >= len then
+	  let pski, bytes = split b len in
+	  match parsePskIdentity pski with
+	  | Correct(id) -> aux bytes (id::ids)
+	  | Error(z) -> Error(z)
+        else Error(AD_decode_error, perror __SOURCE_FILE__ __LINE__ "Failed to parse psk identity length")
+      else Error(AD_decode_error, perror __SOURCE_FILE__ __LINE__ "Expected psk identity to be at least 2 bytes long")
+    else Correct(ids) in
+  match vlparse 2 b with
+  | Correct (b) -> aux b []
+  | Error(z) -> Error(AD_decode_error, perror __SOURCE_FILE__ __LINE__ "Failed to parse psk identities")
+
+type clientPreSharedKey = l:list pskIdentity{List.length l >= 2 /\ List.length l < 65536 }
+type serverPreSharedKey = pskIdentity
+type preSharedKey = 
+  | ClientPreSharedKey of clientPreSharedKey
+  | ServerPreSharedKey of serverPreSharedKey
+
+val clientPreSharedKeyBytes: clientPreSharedKey -> Tot bytes
+let clientPreSharedKeyBytes cpsk = pskIdentitiesBytes cpsk
+
+val parseClientPreSharedKey: pinverse_t clientPreSharedKeyBytes
+let parseClientPreSharedKey b = parsePskIdentities b
+
+val serverPreSharedKeyBytes: serverPreSharedKey -> Tot bytes
+let serverPreSharedKeyBytes cpsk = pskIdentityBytes cpsk
+
+val parseServerPreSharedKey: pinverse_t serverPreSharedKeyBytes
+let parseServerPreSharedKey b = parsePskIdentity b
+
+val preSharedKeyBytes: preSharedKey -> Tot bytes
+let preSharedKeyBytes psk =
+  match psk with
+  | ClientPreSharedKey cpsk -> clientPreSharedKeyBytes cpsk
+  | ServerPreSharedKey spsk -> serverPreSharedKeyBytes spsk
+
+val parsePreSharedKey: pinverse_t preSharedKeyBytes
+let parsePreSharedKey b =
+  match vlparse 2 b with
+  | Correct(b') ->
+      (match vlparse 2 b with
+      | Correct(b'') -> // Client case
+	(match parseClientPreSharedKey b with
+	| Correct(psks) -> Correct(ClientPreSharedKey psks)
+	| Error(z) -> Error(z))
+      | Error(_) -> // Server case
+	(match parseServerPreSharedKey b with
+	| Correct(psk) -> Correct (ServerPreSharedKey psk)
+	| Error(z) -> Error(z)))
+  | Error(z) -> Error(AD_decode_error, perror __SOURCE_FILE__ __LINE__ "Failed to parse pre shared key")
